`SSTORE` opcode equivalence (#7)
* Add `SstoreSummary.lean`

* `SstoreSummary.lean`: prove `EvmYul.step_sstore_summary`

* `KEVM2Lean`: re-generate code

* `ScheduleOrdering`: update according to newly generated code

* `AddEquivalence.lean`: adapt proof to new rewrite label

* `Push0Equivalence.lean`: adapt proof to new rewrite label

* Create `Interfaces/Axioms.lean` file

* `StateMap.lean`: rearrange getters for `SortGeneratedTopCell`

* `StateMap.lean`: Add `KItem` projections to subsorts

* `StateMap.lean`: add several mappings

* `StateMap.lean`: update `stateMap` with more fields

* `FuncInterface.lean`: add behavior for `AccountCellMapItem`

* `AddSummary.lean`: update to reflect `stateMap` changes

* `Push0Summary.lean`: update to reflect `stateMap` changes

* `AddEquivalence.lean`: update to reflect `stateMap` changes

* `Push0Summary.lean`: update to reflect `stateMap` changes

* `Tactics.lean`: add new tactic `simp_flag` for schedule flag reasoning

* `GasInterface.lean`: simplify proof of `neq_gconst_true`

* `GasInterface.lean`: format some `match` arrows `=>`

* `GasInterface.lean`: add interface for `ScheduleFlag` function

* `EvmYulInterface`: add thm `ofNat_toSigned` and section comments

* `FuncInterface`: add interfaces for more functions

These include:
- `==Int` and `=/=Int`
- `kite`
- `in_keys`
- `#inStorage`

* `StateMap`: `set_option linter.deprecated false`

* `StateMap`: tiny improvement to existing comments

* `StateMap`: add `Axioms` on the behavior of the axiomatic state mapping

* `AddSummary`: update for latest state mapping

* `Push0Summary`: update for latest state mapping

* `SstoreSummary`: complete proof of `EVM.step_sstore_summary`

* `AddEquivalence`: update for latest state mapping

* `Push0Equivalence`: update for latest state mapping

* Add `SstoreOpcodeEquivalence.lean`

* `lakefile.toml`: change `defaultTargets` to `EvmEquivalence`

* `EvmEquivalence.lean`: add modules that constitute the project

* `GasInterface.lean`: remove spurious commented theorem

* `SstoreSummary.lean`: prove `X_sstore_summary`

* `StateMap.lean`: add `SortStaticCell` mapping

* Propagate `SortStaticCell` mapping to summaries

* Propagate `SortStaticCell` mapping to `ADD` `PUSH0` `SSTORE` equiv

* `SstoreEquivalence`: add `sstore_gas_pos` theorem

* `SstoreEquivalence`: remove `gas` parameter from `step_sstore_equiv`

* `SstoreEquivalence`: finish `step_sstore_equiv` proof (minus `sorry`)

* `SstoreEquivalence`: prove `X_sstore_equiv` modulo `sorry`

* `SstoreEquivalence.lean`: reorder imports

* `SstoreEquivalence`: comment out proof of `Aᵣ_rsstore_eq`

* `StateMap`: remove variable `ownerAcc` in `accountsCell_map_insert`

* `SstoreEquivalence`: optimize `step_sstore_equiv`; propagate axiom change

* `Interfaces/README.md`: document axioms and axiomatic approach

* `README.md`: update repository structure

* Add `README.md` to `Equivalence` folder

* `Equivalence/README.md`: typos and slight improvements

* `Equivalence/README.md`: typo

* `Equivalence/README.md`: enhancements

EvmEquivalence/Interfaces/FuncInterface.lean
@@ -82,6 +82,10 @@ end -/
 axiom Keq_def (k₁ k₂ : SortK) : «_==K_» k₁ k₂ = some (k₁ == k₂)
 axiom Kneq_def (k₁ k₂ : SortK) : «_=/=K_» k₁ k₂ = some (k₁ != k₂)
 
+-- Behavior of `==Int` and `=/=Int`
+axiom IntEq_def (n m : SortInt) : «_==Int_» n m = some (n == m)
+axiom IntNEq_def (n m : SortInt) : «_=/=Int_» n m = some (n != m)
+
 -- Behavior of `_orBool_` and `_andBool_`
 axiom orBool_def (b₁ b₂ : SortBool) : _orBool_ b₁ b₂ = some (b₁ || b₂)
 axiom andBool_def (b₁ b₂ : SortBool) : _andBool_ b₁ b₂ = some (b₁ && b₂)
@@ -132,5 +136,59 @@ theorem wsLength_eq_length_wordStackMap {ws : SortWordStack} :
 theorem sizeWordStack_def {ws : SortWordStack} :
   sizeWordStackAux ws 0 = some (List.length (wordStackMap ws)) :=
   wsLength_eq_length_wordStackMap ▸ sizeWordStackIsSome
+
+
+-- Behavior of `AccountCellMapItem`
+-- TODO: Complete or delete
+/--
+Note that this function is dependent on the current implementation of `SortAccountCellMap`
+
+The current implementation is `List (SortAcctIDCell × SortAccountCell)` but
+this might change in the future
+-/
+def accountCellMapItem_def (x0 : SortAcctIDCell) (x1 : SortAccountCell) : Option SortAccountCellMap :=
+  some (⟨[(x0, x1)]⟩)
+
+-- Behavior of `kite`
+@[simp]
+theorem kite_def {SortSort : Type} (cnd : SortBool) (true_branch false_branch: SortSort) :
+  kite cnd true_branch false_branch = ite cnd true_branch false_branch := by
+  aesop
+
+-- Behavior of K's `in_keys` function
+-- NOTE: These functions depend on the dummy implementation as maps
+-- being `List (Key × Value)`
+def keys {K V : Type} (l : List (K × V)) : List K :=
+  List.map (λ pair => pair.1) l
+
+def inKeys_compute (map : SortMap) (key : SortInt) : Bool :=
+  List.elem (inj key) (keys map.coll)
+
+@[simp]
+axiom Axioms.inKeys_def (map : SortMap) (key : SortInt) :
+  «_in_keys(_)_MAP_Bool_KItem_Map» (inj ((inj key) : SortAccount)) map =
+  some (inKeys_compute map key)
+
+-- Behavior of `#inStorage`
+noncomputable def inStorage_compute (map : SortMap) (acc key : SortInt) : Bool :=
+  match «Map:lookup» map (inj ((@inj SortInt SortAccount) acc)) with
+  | none => false
+  | some a => match «#inStorageAux1» a key with
+    | none => false
+    | some b => if inKeys_compute map acc then b else false
+
+@[simp]
+theorem inStorage_def {ACCESSEDSTORAGE_CELL : SortMap} {ID_CELL W0 : SortInt} :
+  «#inStorage» ACCESSEDSTORAGE_CELL ((@inj SortInt SortAccount) ID_CELL) W0 = some (inStorage_compute ACCESSEDSTORAGE_CELL ID_CELL W0) := by
+  aesop (add simp [«#inStorage», _dbb1f9e, _8d90a32, Option.bind, inStorage_compute])
+
+-- Helper theorems
+
+@[simp]
+theorem inj_ID_CELL (ID_CELL : SortInt) : @inj SortInt SortAccount instInjSortIntSortAccount ID_CELL = .inj_SortInt ID_CELL := rfl
+
+@[simp]
+theorem accountAddressIsSome (n : ℕ) (size : n < AccountAddress.size) : AccountAddress.ofNat n = ⟨n, size⟩ := by
+  simp [AccountAddress.ofNat, Fin.ofNat]; aesop
 
 end KEVMInterface
