EvmEquivalence/KEVM2Lean/Rewrite.lean
@@ -6,7 +6,7 @@ inductive Rewrites : SortGeneratedTopCell → SortGeneratedTopCell → Prop wher
     (t1 : Rewrites s1 s2)
     (t2 : Rewrites s2 s3)
     : Rewrites s1 s3
-  | SUMMARY_ADD_2_SPEC_BASIC_BLOCK_21_TO_20
+  | ADD_SUMMARY_ADD_SUMMARY_0
     {GAS_CELL PC_CELL W0 W1 _Val0 _Val3 _Val4 _Val5 _Val6 _Val7 : SortInt}
     {K_CELL : SortK}
     {SCHEDULE_CELL : SortSchedule}
@@ -120,7 +120,7 @@ inductive Rewrites : SortGeneratedTopCell → SortGeneratedTopCell → Prop wher
             block := _Gen21 },
           network := _DotVar2 } },
       generatedCounter := _DotVar0 }
-  | SUMMARY_PUSHZERO_0_SPEC_BASIC_BLOCK_25_TO_24
+  | PUSHZERO_SUMMARY_PUSHZERO_SUMMARY_1
     {GAS_CELL PC_CELL _Val0 _Val11 _Val12 _Val13 _Val3 _Val6 : SortInt}
     {K_CELL : SortK}
     {SCHEDULE_CELL : SortSchedule}
@@ -152,17 +152,17 @@ inductive Rewrites : SortGeneratedTopCell → SortGeneratedTopCell → Prop wher
     {_Gen7 : SortMemoryUsedCell}
     {_Gen8 : SortCallGasCell}
     {_Gen9 : SortStaticCell}
-    (defn_Val0 : «_<_>_SCHEDULE_Int_ScheduleConst_Schedule» SortScheduleConst.Gbase_SCHEDULE_ScheduleConst SCHEDULE_CELL = some _Val0)
-    (defn_Val1 : «_<=Int_» _Val0 GAS_CELL = some _Val1)
-    (defn_Val2 : _andBool_ USEGAS_CELL _Val1 = some _Val2)
+    (defn_Val0 : sizeWordStackAux WS 0 = some _Val0)
+    (defn_Val1 : «_<Int_» _Val0 0 = some _Val1)
+    (defn_Val2 : notBool_ _Val1 = some _Val2)
     (defn_Val3 : sizeWordStackAux WS 0 = some _Val3)
-    (defn_Val4 : «_<Int_» _Val3 0 = some _Val4)
+    (defn_Val4 : «_<Int_» 1023 _Val3 = some _Val4)
     (defn_Val5 : notBool_ _Val4 = some _Val5)
-    (defn_Val6 : sizeWordStackAux WS 0 = some _Val6)
-    (defn_Val7 : «_<Int_» 1023 _Val6 = some _Val7)
-    (defn_Val8 : notBool_ _Val7 = some _Val8)
-    (defn_Val9 : _andBool_ _Val5 _Val8 = some _Val9)
-    (defn_Val10 : _andBool_ _Val2 _Val9 = some _Val10)
+    (defn_Val6 : «_<_>_SCHEDULE_Int_ScheduleConst_Schedule» SortScheduleConst.Gbase_SCHEDULE_ScheduleConst SCHEDULE_CELL = some _Val6)
+    (defn_Val7 : «_<=Int_» _Val6 GAS_CELL = some _Val7)
+    (defn_Val8 : _andBool_ _Val5 _Val7 = some _Val8)
+    (defn_Val9 : _andBool_ _Val2 _Val8 = some _Val9)
+    (defn_Val10 : _andBool_ USEGAS_CELL _Val9 = some _Val10)
     (defn_Val11 : «_+Int_» PC_CELL 1 = some _Val11)
     (defn_Val12 : «_<_>_SCHEDULE_Int_ScheduleConst_Schedule» SortScheduleConst.Gbase_SCHEDULE_ScheduleConst SCHEDULE_CELL = some _Val12)
     (defn_Val13 : «_-Int_» GAS_CELL _Val12 = some _Val13)
@@ -239,4 +239,210 @@ inductive Rewrites : SortGeneratedTopCell → SortGeneratedTopCell → Prop wher
             blockhashes := _Gen20,
             block := _Gen21 },
           network := _DotVar2 } },
+      generatedCounter := _DotVar0 }
+  | SSTORE_SUMMARY_SSTORE_SUMMARY_1
+    {ACCESSEDSTORAGE_CELL ORIG_STORAGE_CELL STORAGE_CELL _Val39 _Val40 : SortMap}
+    {GAS_CELL ID_CELL PC_CELL REFUND_CELL W0 W1 _Val1 _Val10 _Val11 _Val13 _Val2 _Val21 _Val22 _Val23 _Val24 _Val25 _Val27 _Val28 _Val29 _Val3 _Val30 _Val31 _Val32 _Val33 _Val6 _Val7 _Val8 _Val9 : SortInt}
+    {K_CELL : SortK}
+    {SCHEDULE_CELL : SortSchedule}
+    {USEGAS_CELL _Val0 _Val12 _Val14 _Val15 _Val16 _Val17 _Val18 _Val26 _Val4 _Val5 : SortBool}
+    {WS : SortWordStack}
+    {_DotVar0 : SortGeneratedCounterCell}
+    {_DotVar6 _Val19 _Val20 _Val41 _Val42 : SortAccountCellMap}
+    {_Gen0 : SortProgramCell}
+    {_Gen1 : SortJumpDestsCell}
+    {_Gen10 : SortLogCell}
+    {_Gen11 : SortAccessedAccountsCell}
+    {_Gen12 : SortCreatedAccountsCell}
+    {_Gen13 : SortOutputCell}
+    {_Gen14 : SortStatusCodeCell}
+    {_Gen15 : SortCallStackCell}
+    {_Gen16 : SortInterimStatesCell}
+    {_Gen17 : SortTouchedAccountsCell}
+    {_Gen18 : SortVersionedHashesCell}
+    {_Gen19 : SortGasPriceCell}
+    {_Gen2 : SortCallerCell}
+    {_Gen20 : SortOriginCell}
+    {_Gen21 : SortBlockhashesCell}
+    {_Gen22 : SortBlockCell}
+    {_Gen23 : SortBalanceCell}
+    {_Gen24 : SortCodeCell}
+    {_Gen25 : SortTransientStorageCell}
+    {_Gen26 : SortNonceCell}
+    {_Gen27 : SortChainIDCell}
+    {_Gen28 : SortTxOrderCell}
+    {_Gen29 : SortTxPendingCell}
+    {_Gen3 : SortCallDataCell}
+    {_Gen30 : SortMessagesCell}
+    {_Gen31 : SortWithdrawalsPendingCell}
+    {_Gen32 : SortWithdrawalsOrderCell}
+    {_Gen33 : SortWithdrawalsCell}
+    {_Gen34 : SortExitCodeCell}
+    {_Gen35 : SortModeCell}
+    {_Gen4 : SortCallValueCell}
+    {_Gen5 : SortLocalMemCell}
+    {_Gen6 : SortMemoryUsedCell}
+    {_Gen7 : SortCallGasCell}
+    {_Gen8 : SortCallDepthCell}
+    {_Gen9 : SortSelfDestructCell}
+    {_Val34 _Val36 _Val37 _Val38 : SortSet}
+    {_Val35 : SortKItem}
+    (defn_Val0 : «_<<_>>_SCHEDULE_Bool_ScheduleFlag_Schedule» SortScheduleFlag.Ghasaccesslist_SCHEDULE_ScheduleFlag SCHEDULE_CELL = some _Val0)
+    (defn_Val1 : lookup STORAGE_CELL W0 = some _Val1)
+    (defn_Val2 : lookup ORIG_STORAGE_CELL W0 = some _Val2)
+    (defn_Val3 : Csstore SCHEDULE_CELL W1 _Val1 _Val2 = some _Val3)
+    (defn_Val4 : «_<=Int_» _Val3 GAS_CELL = some _Val4)
+    (defn_Val5 : «#inStorage» ACCESSEDSTORAGE_CELL ((@inj SortInt SortAccount) ID_CELL) W0 = some _Val5)
+    (defn_Val6 : «_<_>_SCHEDULE_Int_ScheduleConst_Schedule» SortScheduleConst.Gcoldsload_SCHEDULE_ScheduleConst SCHEDULE_CELL = some _Val6)
+    (defn_Val7 : kite _Val5 0 _Val6 = some _Val7)
+    (defn_Val8 : lookup STORAGE_CELL W0 = some _Val8)
+    (defn_Val9 : lookup ORIG_STORAGE_CELL W0 = some _Val9)
+    (defn_Val10 : Csstore SCHEDULE_CELL W1 _Val8 _Val9 = some _Val10)
+    (defn_Val11 : «_-Int_» GAS_CELL _Val10 = some _Val11)
+    (defn_Val12 : «_<=Int_» _Val7 _Val11 = some _Val12)
+    (defn_Val13 : «_<_>_SCHEDULE_Int_ScheduleConst_Schedule» SortScheduleConst.Gcallstipend_SCHEDULE_ScheduleConst SCHEDULE_CELL = some _Val13)
+    (defn_Val14 : «_<Int_» _Val13 GAS_CELL = some _Val14)
+    (defn_Val15 : _andBool_ _Val12 _Val14 = some _Val15)
+    (defn_Val16 : _andBool_ _Val4 _Val15 = some _Val16)
+    (defn_Val17 : _andBool_ _Val0 _Val16 = some _Val17)
+    (defn_Val18 : _andBool_ USEGAS_CELL _Val17 = some _Val18)
+    (defn_Val19 : AccountCellMapItem { val := ID_CELL } {
+      acctID := { val := ID_CELL },
+      balance := _Gen23,
+      code := _Gen24,
+      storage := { val := STORAGE_CELL },
+      origStorage := { val := ORIG_STORAGE_CELL },
+      transientStorage := _Gen25,
+      nonce := _Gen26 } = some _Val19)
+    (defn_Val20 : _AccountCellMap_ _Val19 _DotVar6 = some _Val20)
+    (defn_Val21 : «_+Int_» PC_CELL 1 = some _Val21)
+    (defn_Val22 : lookup STORAGE_CELL W0 = some _Val22)
+    (defn_Val23 : lookup ORIG_STORAGE_CELL W0 = some _Val23)
+    (defn_Val24 : Csstore SCHEDULE_CELL W1 _Val22 _Val23 = some _Val24)
+    (defn_Val25 : «_-Int_» GAS_CELL _Val24 = some _Val25)
+    (defn_Val26 : «#inStorage» ACCESSEDSTORAGE_CELL ((@inj SortInt SortAccount) ID_CELL) W0 = some _Val26)
+    (defn_Val27 : «_<_>_SCHEDULE_Int_ScheduleConst_Schedule» SortScheduleConst.Gcoldsload_SCHEDULE_ScheduleConst SCHEDULE_CELL = some _Val27)
+    (defn_Val28 : kite _Val26 0 _Val27 = some _Val28)
+    (defn_Val29 : «_-Int_» _Val25 _Val28 = some _Val29)
+    (defn_Val30 : lookup STORAGE_CELL W0 = some _Val30)
+    (defn_Val31 : lookup ORIG_STORAGE_CELL W0 = some _Val31)
+    (defn_Val32 : Rsstore SCHEDULE_CELL W1 _Val30 _Val31 = some _Val32)
+    (defn_Val33 : «_+Int_» REFUND_CELL _Val32 = some _Val33)
+    (defn_Val34 : «.Set» = some _Val34)
+    (defn_Val35 : «Map:lookupOrDefault» ACCESSEDSTORAGE_CELL ((@inj SortInt SortKItem) ID_CELL) ((@inj SortSet SortKItem) _Val34) = some _Val35)
+    (defn_Val36 : «project:Set» (SortK.kseq _Val35 SortK.dotk) = some _Val36)
+    (defn_Val37 : SetItem ((@inj SortInt SortKItem) W0) = some _Val37)
+    (defn_Val38 : «_|Set__SET_Set_Set_Set» _Val36 _Val37 = some _Val38)
+    (defn_Val39 : «Map:update» ACCESSEDSTORAGE_CELL ((@inj SortInt SortKItem) ID_CELL) ((@inj SortSet SortKItem) _Val38) = some _Val39)
+    (defn_Val40 : «Map:update» STORAGE_CELL ((@inj SortInt SortKItem) W0) ((@inj SortInt SortKItem) W1) = some _Val40)
+    (defn_Val41 : AccountCellMapItem { val := ID_CELL } {
+      acctID := { val := ID_CELL },
+      balance := _Gen23,
+      code := _Gen24,
+      storage := { val := _Val40 },
+      origStorage := { val := ORIG_STORAGE_CELL },
+      transientStorage := _Gen25,
+      nonce := _Gen26 } = some _Val41)
+    (defn_Val42 : _AccountCellMap_ _Val41 _DotVar6 = some _Val42)
+    (req : _Val18 = true)
+    : Rewrites {
+      kevm := {
+        k := { val := SortK.kseq ((@inj SortInternalOp SortKItem) (SortInternalOp.«#next[_]_EVM_InternalOp_MaybeOpCode» ((@inj SortBinStackOp SortMaybeOpCode) SortBinStackOp.SSTORE_EVM_BinStackOp))) K_CELL },
+        exitCode := _Gen34,
+        mode := _Gen35,
+        schedule := { val := SCHEDULE_CELL },
+        useGas := { val := USEGAS_CELL },
+        ethereum := {
+          evm := {
+            output := _Gen13,
+            statusCode := _Gen14,
+            callStack := _Gen15,
+            interimStates := _Gen16,
+            touchedAccounts := _Gen17,
+            callState := {
+              program := _Gen0,
+              jumpDests := _Gen1,
+              id := { val := (@inj SortInt SortAccount) ID_CELL },
+              caller := _Gen2,
+              callData := _Gen3,
+              callValue := _Gen4,
+              wordStack := { val := SortWordStack.«_:__EVM-TYPES_WordStack_Int_WordStack» W0 (SortWordStack.«_:__EVM-TYPES_WordStack_Int_WordStack» W1 WS) },
+              localMem := _Gen5,
+              pc := { val := PC_CELL },
+              gas := { val := (@inj SortInt SortGas) GAS_CELL },
+              memoryUsed := _Gen6,
+              callGas := _Gen7,
+              static := { val := false },
+              callDepth := _Gen8 },
+            versionedHashes := _Gen18,
+            substate := {
+              selfDestruct := _Gen9,
+              log := _Gen10,
+              refund := { val := REFUND_CELL },
+              accessedAccounts := _Gen11,
+              accessedStorage := { val := ACCESSEDSTORAGE_CELL },
+              createdAccounts := _Gen12 },
+            gasPrice := _Gen19,
+            origin := _Gen20,
+            blockhashes := _Gen21,
+            block := _Gen22 },
+          network := {
+            chainID := _Gen27,
+            accounts := { val := _Val20 },
+            txOrder := _Gen28,
+            txPending := _Gen29,
+            messages := _Gen30,
+            withdrawalsPending := _Gen31,
+            withdrawalsOrder := _Gen32,
+            withdrawals := _Gen33 } } },
+      generatedCounter := _DotVar0 } {
+      kevm := {
+        k := { val := K_CELL },
+        exitCode := _Gen34,
+        mode := _Gen35,
+        schedule := { val := SCHEDULE_CELL },
+        useGas := { val := true },
+        ethereum := {
+          evm := {
+            output := _Gen13,
+            statusCode := _Gen14,
+            callStack := _Gen15,
+            interimStates := _Gen16,
+            touchedAccounts := _Gen17,
+            callState := {
+              program := _Gen0,
+              jumpDests := _Gen1,
+              id := { val := (@inj SortInt SortAccount) ID_CELL },
+              caller := _Gen2,
+              callData := _Gen3,
+              callValue := _Gen4,
+              wordStack := { val := WS },
+              localMem := _Gen5,
+              pc := { val := _Val21 },
+              gas := { val := (@inj SortInt SortGas) _Val29 },
+              memoryUsed := _Gen6,
+              callGas := _Gen7,
+              static := { val := false },
+              callDepth := _Gen8 },
+            versionedHashes := _Gen18,
+            substate := {
+              selfDestruct := _Gen9,
+              log := _Gen10,
+              refund := { val := _Val33 },
+              accessedAccounts := _Gen11,
+              accessedStorage := { val := _Val39 },
+              createdAccounts := _Gen12 },
+            gasPrice := _Gen19,
+            origin := _Gen20,
+            blockhashes := _Gen21,
+            block := _Gen22 },
+          network := {
+            chainID := _Gen27,
+            accounts := { val := _Val42 },
+            txOrder := _Gen28,
+            txPending := _Gen29,
+            messages := _Gen30,
+            withdrawalsPending := _Gen31,
+            withdrawalsOrder := _Gen32,
+            withdrawals := _Gen33 } } },
       generatedCounter := _DotVar0 }
