EvmEquivalence/StateMap.lean
@@ -4,10 +4,75 @@ import EvmEquivalence.KEVM2Lean.Inj
 import EvmEquivalence.KEVM2Lean.Func
 import EvmEquivalence.KEVM2Lean.Rewrite
 import EvmEquivalence.Interfaces.EvmYulInterface
+import EvmEquivalence.Interfaces.Axioms
 import EvmEquivalence.Utils.IntUtils
 
 open EvmYul
 open EVM
+
+set_option linter.deprecated false
+
+/- Getters for accessing cells from the Generated Top Cell -/
+
+namespace SortGeneratedTopCell
+
+variable (tc : SortGeneratedTopCell)
+
+@[simp]
+def evm :SortEvmCell := tc.kevm.ethereum.evm
+
+@[simp]
+def callState : SortCallStateCell := tc.kevm.ethereum.evm.callState
+
+@[simp]
+def wordStackCell : SortWordStackCell := tc.kevm.ethereum.evm.callState.wordStack
+
+@[simp]
+def pc : SortPcCell := tc.kevm.ethereum.evm.callState.pc
+
+@[simp]
+def gas : SortGasCell := tc.kevm.ethereum.evm.callState.gas
+
+@[simp]
+def program : SortProgramCell := tc.kevm.ethereum.evm.callState.program
+
+@[simp]
+def output : SortOutputCell := tc.kevm.ethereum.evm.output
+
+@[simp]
+def accessedStorage : SortAccessedStorageCell := tc.kevm.ethereum.evm.substate.accessedStorage
+
+@[simp]
+def refund : SortRefundCell := tc.kevm.ethereum.evm.substate.refund
+
+@[simp]
+def accounts : SortAccountsCell := tc.kevm.ethereum.network.accounts
+
+@[simp]
+def Iₐ : SortIdCell := tc.kevm.ethereum.evm.callState.id
+
+@[simp]
+def isStatic : SortStaticCell := tc.kevm.ethereum.evm.callState.static
+
+end SortGeneratedTopCell
+
+namespace SortKItem
+
+/- KItem projections to subsorts -/
+@[simp]
+def toAccountSort (k : SortKItem) : Option SortAccount :=
+  match k with
+  | .inj_SortAccount acc => some acc
+  | _ => none
+
+/- Subsort projections to KItem -/
+@[simp]
+def ofAccountSort(acc : SortAccount) : SortKItem :=
+  SortKItem.inj_SortAccount acc
+
+end SortKItem
+
+open SortKItem
 
 namespace StateMap
 
@@ -36,44 +101,67 @@ def gasMap (gs : SortGas) : UInt256 :=
 def gasCellMap (gc : SortGasCell) : UInt256 :=
   gasMap gc.val
 
-/- Getters for accessing cells from the Generated Top Cell -/
+@[simp]
+def accountAddressMap (acc : SortAccount) : AccountAddress :=
+  match acc with
+  | .«.Account_EVM-TYPES_Account» => 0
+  | .inj_SortInt n => AccountAddress.ofNat (Int.toNat n)
 
 @[simp]
-def evmOfGTC (tc : SortGeneratedTopCell) :SortEvmCell :=
-  tc.kevm.ethereum.evm
+def idMap (idc : SortIdCell) : AccountAddress :=
+  accountAddressMap idc.val
 
 @[simp]
-def callStateOfGTC (tc : SortGeneratedTopCell) : SortCallStateCell :=
-  tc.kevm.ethereum.evm.callState
+def acctIDMap (aid : SortAcctIDCell) : AccountAddress :=
+  AccountAddress.ofNat (Int.toNat aid.val)
 
 @[simp]
-def wordStackCellOfGTC (tc : SortGeneratedTopCell) : SortWordStackCell :=
-  tc.kevm.ethereum.evm.callState.wordStack
+noncomputable def storageMap (stor : SortStorageCell) : Storage :=
+  Axioms.SortStorageCellMap stor
 
 @[simp]
-def pcOfGTC (tc : SortGeneratedTopCell) : SortPcCell :=
-  tc.kevm.ethereum.evm.callState.pc
+noncomputable def transStorageMap (tstor : SortTransientStorageCell) : Storage :=
+  Axioms.SortTransientStorageCellMap tstor
 
 @[simp]
-def gasOfGTC (tc : SortGeneratedTopCell) : SortGasCell :=
-  tc.kevm.ethereum.evm.callState.gas
-@[simp]
-def programOfGTC (tc : SortGeneratedTopCell) : SortProgramCell :=
-  tc.kevm.ethereum.evm.callState.program
-@[simp]
-def outputOfGTC (tc : SortGeneratedTopCell) : SortOutputCell :=
-  tc.kevm.ethereum.evm.output
+def accCodeMap (code : SortAccountCode) : ByteArray :=
+  match code with | SortAccountCode.inj_SortBytes code => code
 
-/- State Mapping: Mapping KEVM states to EvmYul states -/
+/- Note that Origin Storage Cell (`origStorage`) is not needed from `SortAccountCell` -/
+@[simp]
+noncomputable def accountMap (acc : SortAccountCell) : Account where
+  nonce := intMap acc.nonce.val
+  balance := intMap acc.balance.val
+  storage := storageMap acc.storage
+  code := accCodeMap acc.code.val
+  tstorage := transStorageMap acc.transientStorage
 
--- We temporarely require the `symState` argument since we don't map the entire KEVM state yet
-def stateMap (symState : EVM.State) (tc : SortGeneratedTopCell) : EVM.State :=
+/--
+**State Mapping**: Mapping KEVM states to EvmYul states
+
+We temporarely require the `symState` argument since we don't map the entire KEVM state yet
+
+The following data structures are axiomatically mapped:
+1. `Substate.accessedStorageKeys`:
+  The `EvmYul` data representation for this is an `RBSet`, which is hard to reason about.
+  The mapping will remain an axiom until a better reasoning interface is provided or we have time to implement it
+2. `State.accountMap`: Similar reasons as above
+-/
+noncomputable def stateMap (symState : EVM.State) (tc : SortGeneratedTopCell) : EVM.State :=
   {symState with
-  stack := wordStackCellMap (wordStackCellOfGTC tc)
-  pc := pcCellMap (pcOfGTC tc)
-  gasAvailable := gasCellMap (gasOfGTC tc)
-  executionEnv := {symState.executionEnv with code := (programOfGTC tc).val}
-  returnData := (outputOfGTC tc).val
+  stack := wordStackCellMap tc.wordStackCell
+  pc := pcCellMap tc.pc
+  gasAvailable := gasCellMap tc.gas
+  executionEnv := {symState.executionEnv with
+                code := tc.program.val,
+                codeOwner := idMap tc.Iₐ
+                perm := !tc.isStatic.val}
+  accountMap := Axioms.SortAccountsCellMap tc.accounts
+  substate := {symState.substate with
+            accessedStorageKeys :=  Axioms.SortAccessedStorageCellMap tc.accessedStorage
+            refundBalance := intMap tc.refund.val
+           }
+  returnData := tc.output.val
   }
 
 /- State Mapping Results -/
@@ -115,3 +203,148 @@ theorem intMap_toNat {n : SortInt} (nh : 0 ≤ n) (size : n < UInt256.size) :
   aesop (add simp [intMap, Int.toNat, UInt256.toSigned, Int.toNat_ofNat, UInt256.ofNat_toNat])
 
 end StateMap
+
+open StateMap
+
+namespace Axioms
+
+/--
+This axiom states that if an account is in an `AccountCellMap`, then
+`Batteries.RBMap.find?` finds it in the image of the axiomatized mapping
+
+The second element of `AccountCellMapItem` is provided embedded in `accCellMap_def` for
+ease of use when proving theorems
+ -/
+axiom findAccountInAccountCellMap
+  {ID_CELL : SortInt}
+  {balance : SortBalanceCell}
+  {code : SortCodeCell}
+  {STORAGE_CELL ORIG_STORAGE_CELL : SortMap}
+  {tstorage : SortTransientStorageCell}
+  {nonce : SortNonceCell}
+  {accCellMap dotVar accCellMap2 : SortAccountCellMap}
+  (accCellMap_def : AccountCellMapItem { val := ID_CELL } {
+    acctID := { val := ID_CELL },
+    balance := balance,
+    code := code,
+    storage := { val := STORAGE_CELL },
+    origStorage := { val := ORIG_STORAGE_CELL },
+    transientStorage := tstorage,
+    nonce := nonce } = some accCellMap)
+  (accCellMap2_def : _AccountCellMap_ accCellMap dotVar = some accCellMap2) :
+  Batteries.RBMap.find? (Axioms.SortAccountsCellMap { val := accCellMap2 }) (AccountAddress.ofNat (Int.toNat ID_CELL)) = some (StateMap.accountMap {
+    acctID := { val := ID_CELL },
+    balance := balance,
+    code := code,
+    storage := { val := STORAGE_CELL },
+    origStorage := { val := ORIG_STORAGE_CELL },
+    transientStorage := tstorage,
+    nonce := nonce })
+
+/--
+Expected behavior of `SortAccountsCellMap` w.r.t. `Batteries.RBMap.find?`
+
+This axiom states that
+- Given an `accountsCell` (`accCellMap2`) containing an account identifiable by `ID_CELL` (`acc`)
+- The (axiomatic) mapping of `accCellMap2` contains the mapping of `acc`
+- And, in particular, `RBMap.find?` correctly finds the mapped `acc` if provided with the mapped `ID_CELL`
+ -/
+axiom accountsCell_map_find?
+  {ID_CELL : SortInt}
+  {balance : SortBalanceCell}
+  {code : SortCodeCell}
+  {STORAGE_CELL ORIG_STORAGE_CELL : SortMap}
+  {tstorage : SortTransientStorageCell}
+  {nonce : SortNonceCell}
+  {accCellMap dotVar accCellMap2 : SortAccountCellMap}
+  (acc : SortAccountCell)
+  (acc_def : acc = {
+    acctID := { val := ID_CELL },
+    balance := balance,
+    code := code,
+    storage := { val := STORAGE_CELL },
+    origStorage := { val := ORIG_STORAGE_CELL },
+    transientStorage := tstorage,
+    nonce := nonce })
+  (accCellMap_def : AccountCellMapItem { val := ID_CELL } acc = some accCellMap)
+  (accCellMap2_def : _AccountCellMap_ accCellMap dotVar = some accCellMap2) :
+  Batteries.RBMap.find? (Axioms.SortAccountsCellMap { val := accCellMap2 }) (AccountAddress.ofNat (Int.toNat ID_CELL)) = some (StateMap.accountMap acc)
+
+/--
+Expected behavior of `SortAccountsCellMap` w.r.t. `Batteries.RBMap.insert`
+
+This axiom states that
+- Given an `accountsCell` (`initCellMap`) containing an account identifiable by `ID_CELL` (`initAccount`) with symbolic storage `STORAGE_CELL`
+- Given an updated `accountsCell` (`updatedCellMap`) consisting of `initAccount` with an updated `STORAGE_CELL` which contains the symbolic (`key`, `value`) pair (`stor_update`)
+- `RBMap.insert`ing the mapped (`key`, `value`) pair into the (axiomatically) mapped `initCellMap` equals to the (axiomatic) mapping of `updatedCellMap`
+ -/
+axiom accountsCell_map_insert
+  {ID_CELL key value : SortInt}
+  {balance : SortBalanceCell}
+  {code : SortCodeCell}
+  {tstorage : SortTransientStorageCell}
+  {nonce : SortNonceCell}
+  {ACCESSEDSTORAGE_CELL ORIG_STORAGE_CELL STORAGE_CELL stor_update : SortMap}
+  {emptySet kitemToSet keySet fullSet : SortSet}
+  {kitemLookup : SortKItem}
+  {dotvar initAccount initCellMap updatedAccount updatedCellMap : SortAccountCellMap}
+  (defn_Val34 : «.Set» = some emptySet)
+  (defn_Val35 : «Map:lookupOrDefault» ACCESSEDSTORAGE_CELL ((@inj SortInt SortKItem) ID_CELL) ((@inj SortSet SortKItem) emptySet) = some kitemLookup)
+  (defn_Val36 : «project:Set» (SortK.kseq kitemLookup SortK.dotk) = some kitemToSet)
+  (defn_Val37 : SetItem ((@inj SortInt SortKItem) key) = some keySet)
+  (defn_Val38 : «_|Set__SET_Set_Set_Set» kitemToSet keySet = some fullSet)
+  (defn_Val40 : «Map:update» STORAGE_CELL ((@inj SortInt SortKItem) key) ((@inj SortInt SortKItem) value) = some stor_update)
+  (defn_Val41 : AccountCellMapItem { val := ID_CELL } {
+    acctID := { val := ID_CELL },
+    balance := balance,
+    code := code,
+    storage := { val := stor_update },
+    origStorage := { val := ORIG_STORAGE_CELL },
+    transientStorage := tstorage,
+    nonce := nonce } = some updatedAccount)
+  (defn_Val42 : _AccountCellMap_ updatedAccount dotvar = some updatedCellMap)
+  (defn_Val19 : AccountCellMapItem { val := ID_CELL } {
+    acctID := { val := ID_CELL },
+    balance := balance,
+    code := code,
+    storage := { val := STORAGE_CELL },
+    origStorage := { val := ORIG_STORAGE_CELL },
+    transientStorage := tstorage,
+    nonce := nonce } = some initAccount)
+  (defn_Val20 : _AccountCellMap_ initAccount dotvar = some initCellMap)
+  :
+  Batteries.RBMap.insert (Axioms.SortAccountsCellMap { val := initCellMap }) (accountAddressMap (inj ID_CELL))
+    ((accountMap {
+    acctID := { val := ID_CELL },
+    balance := balance,
+    code := code,
+    storage := { val := STORAGE_CELL },
+    origStorage := { val := ORIG_STORAGE_CELL },
+    transientStorage := tstorage,
+    nonce := nonce }).updateStorage (intMap key) (intMap value)) =
+  Axioms.SortAccountsCellMap { val := updatedCellMap }
+
+/--
+Expected behavior of `SortAccessedStorageCellMap` w.r.t. `Batteries.RBSet.insert`
+
+This axiom states that
+- Given a symbolic map of accessed storage keys `ACCESSEDSTORAGE_CELL`
+- Given an update of `ACCESSEDSTORAGE_CELL` containing the account `ID_CELL` and the key `key` (`stor_update`)
+- `RBMap.insert`ing the mapped pair (`ID_CELL`, `key`) into the (axiomatically) mapped `ACCESSEDSTORAGE_CELL` equals to the (axiomatic) mapping of `stor_update`
+ -/
+axiom accessedStorageCell_map_insert
+    {ID_CELL key : SortInt}
+  {ACCESSEDSTORAGE_CELL stor_update : SortMap}
+  {emptySet kitemToSet keySet fullSet : SortSet}
+  {kitemLookup : SortKItem}
+  (defn_Val34 : «.Set» = some emptySet)
+  (defn_Val35 : «Map:lookupOrDefault» ACCESSEDSTORAGE_CELL ((@inj SortInt SortKItem) ID_CELL) ((@inj SortSet SortKItem) emptySet) = some kitemLookup)
+  (defn_Val36 : «project:Set» (SortK.kseq kitemLookup SortK.dotk) = some kitemToSet)
+  (defn_Val37 : SetItem ((@inj SortInt SortKItem) key) = some keySet)
+  (defn_Val38 : «_|Set__SET_Set_Set_Set» kitemToSet keySet = some fullSet)
+  (defn_Val39 : «Map:update» ACCESSEDSTORAGE_CELL ((@inj SortInt SortKItem) ID_CELL) ((@inj SortSet SortKItem) fullSet) = some stor_update) :
+  (Axioms.SortAccessedStorageCellMap { val := ACCESSEDSTORAGE_CELL }).insert
+    (AccountAddress.ofNat (Int.toNat ID_CELL), intMap key) =
+  Axioms.SortAccessedStorageCellMap { val := stor_update }
+
+end Axioms
