EvmEquivalence/Equivalence/AddEquivalence.lean
@@ -192,7 +192,7 @@ theorem rw_addLHS_addRHS
   Rewrites
   (@addLHS GAS_CELL PC_CELL W0 W1 K_CELL SCHEDULE_CELL USEGAS_CELL WS _DotVar0 _DotVar2 _Gen0 _Gen1 _Gen10 _Gen11 _Gen12 _Gen13 _Gen14 _Gen15 _Gen16 _Gen17 _Gen18 _Gen19 _Gen2 _Gen20 _Gen21 _Gen22 _Gen23 _Gen3 _Gen4 _Gen5 _Gen6 _Gen7 _Gen8 _Gen9)
   (@addRHS _Val0 _Val3 _Val4 _Val5 _Val6 _Val7 K_CELL SCHEDULE_CELL _Val1 _Val2 WS _DotVar0 _DotVar2 _Gen0 _Gen1 _Gen10 _Gen11 _Gen12 _Gen13 _Gen14 _Gen15 _Gen16 _Gen17 _Gen18 _Gen19 _Gen2 _Gen20 _Gen21 _Gen22 _Gen23 _Gen3 _Gen4 _Gen5 _Gen6 _Gen7 _Gen8 _Gen9) := by
-  apply Rewrites.SUMMARY_ADD_2_SPEC_BASIC_BLOCK_21_TO_20 <;> try assumption
+  apply Rewrites.ADD_SUMMARY_ADD_SUMMARY_0 <;> try assumption
   simp_all
 
 theorem add_prestate_equiv
@@ -228,12 +228,21 @@ theorem add_prestate_equiv
   {_Gen8 : SortCallGasCell}
   {_Gen9 : SortStaticCell}
   (symState : EVM.State):
-  stateMap symState (@addLHS GAS_CELL PC_CELL W0 W1 K_CELL SCHEDULE_CELL USEGAS_CELL WS _DotVar0 _DotVar2 _Gen0 _Gen1 _Gen10 _Gen11 _Gen12 _Gen13 _Gen14 _Gen15 _Gen16 _Gen17 _Gen18 _Gen19 _Gen2 _Gen20 _Gen21 _Gen22 _Gen23 _Gen3 _Gen4 _Gen5 _Gen6 _Gen7 _Gen8 _Gen9) =
+  let lhs := (@addLHS GAS_CELL PC_CELL W0 W1 K_CELL SCHEDULE_CELL USEGAS_CELL WS _DotVar0 _DotVar2 _Gen0 _Gen1 _Gen10 _Gen11 _Gen12 _Gen13 _Gen14 _Gen15 _Gen16 _Gen17 _Gen18 _Gen19 _Gen2 _Gen20 _Gen21 _Gen22 _Gen23 _Gen3 _Gen4 _Gen5 _Gen6 _Gen7 _Gen8 _Gen9)
+  stateMap symState lhs =
   {symState with
     stack := (intMap W0) :: (intMap W1) :: wordStackMap WS
     pc := intMap PC_CELL
     gasAvailable := intMap GAS_CELL
-    executionEnv := {symState.executionEnv with code := _Gen0.val}
+    executionEnv := {symState.executionEnv with
+                  code := _Gen0.val,
+                  codeOwner := idMap lhs.Iₐ
+                  perm := !lhs.isStatic.val}
+    accountMap := Axioms.SortAccountsCellMap lhs.accounts
+    substate := {symState.substate with
+            accessedStorageKeys :=  Axioms.SortAccessedStorageCellMap lhs.accessedStorage
+            refundBalance := intMap _Gen17.refund.val
+           }
     returnData := _Gen11.val
     } := rfl
 
@@ -273,14 +282,24 @@ theorem add_poststate_equiv
   (defn_Val4 : chop _Val3 = some _Val4)
   (defn_Val5 : «_+Int_» PC_CELL 1 = some _Val5)
   (symState : EVM.State):
-  stateMap symState (@addRHS _Val0 _Val3 _Val4 _Val5 _Val6 _Val7 K_CELL SCHEDULE_CELL _Val1 _Val2 WS _DotVar0 _DotVar2 _Gen0 _Gen1 _Gen10 _Gen11 _Gen12 _Gen13 _Gen14 _Gen15 _Gen16 _Gen17 _Gen18 _Gen19 _Gen2 _Gen20 _Gen21 _Gen22 _Gen23 _Gen3 _Gen4 _Gen5 _Gen6 _Gen7 _Gen8 _Gen9) =
+  let rhs := (@addRHS _Val0 _Val3 _Val4 _Val5 _Val6 _Val7 K_CELL SCHEDULE_CELL _Val1 _Val2 WS _DotVar0 _DotVar2 _Gen0 _Gen1 _Gen10 _Gen11 _Gen12 _Gen13 _Gen14 _Gen15 _Gen16 _Gen17 _Gen18 _Gen19 _Gen2 _Gen20 _Gen21 _Gen22 _Gen23 _Gen3 _Gen4 _Gen5 _Gen6 _Gen7 _Gen8 _Gen9)
+  stateMap symState rhs =
   {symState with
     stack := (intMap (chop' («_+Int'_» W0 W1))) :: wordStackMap WS
     pc := intMap («_+Int'_» PC_CELL 1)
     gasAvailable := intMap _Val7
-    executionEnv := {symState.executionEnv with code := _Gen0.val}
+    executionEnv := {symState.executionEnv with
+                  code := _Gen0.val,
+                  codeOwner := idMap rhs.Iₐ,
+                  perm := !rhs.isStatic.val}
+    accountMap := Axioms.SortAccountsCellMap rhs.accounts
+    substate := {symState.substate with
+            accessedStorageKeys :=  Axioms.SortAccessedStorageCellMap rhs.accessedStorage
+            refundBalance := intMap _Gen17.refund.val
+           }
     returnData := _Gen11.val
     } := by aesop (add simp [«_+Int'_», chop'])
+
 
 open AddSummary
 
@@ -346,7 +365,7 @@ theorem step_add_equiv
   cases gas; contradiction
   case succ gas =>
     rw [EVM.step_add_summary] <;> try assumption
-    congr
+    simp [addLHS, addRHS]; constructor <;> try constructor
     . aesop (add simp [GasInterface.cancun_def, «_-Int_», intMap_sub_dist])
     . rw [plusInt_def, ←UInt256.add_succ_mod_size, intMap_add_dist] <;> aesop
     . aesop (add simp [intMap, chop_def, plusInt_def, intMap_add_dist])
@@ -418,7 +437,7 @@ theorem X_add_equiv
   -- If we don't apply this lemma we cannot rewrite X_add_summary
   have pc_equiv : intMap 0 = UInt256.ofNat 0 := rfl
   rw [pc_equiv, X_add_summary]
-  · aesop (add simp [GasInterface.cancun_def, «_-Int_», chop_def, plusInt_def, intMap_add_dist])
+  · aesop (add simp [GasInterface.cancun_def, «_-Int_», chop_def, plusInt_def, intMap_add_dist, addLHS, addRHS])
       (add safe (by rw [intMap_sub_dist])) (add safe (by apply le_of_lt))
   · aesop (add simp [GasConstants.Gverylow, intMap, UInt256.toSigned])
       (add simp [intMap_toNat, UInt256.ofNat_toNat])
