EvmEquivalence/Summaries/AddSummary.lean
@@ -14,10 +14,13 @@ section
 variable (word₁ word₂ : UInt256)
 variable (gas gasCost : ℕ)
 variable (symStack : Stack UInt256)
-variable (symPc : UInt256)
-variable (symGasAvailable : UInt256)
+variable (symPc symGasAvailable symRefund : UInt256)
 variable (symExecLength : ℕ)
 variable (symReturnData symCode : ByteArray)
+variable (symAccessedStorageKeys : Batteries.RBSet (AccountAddress × UInt256) Substate.storageKeysCmp)
+variable (symAccounts : AccountMap)
+variable (symCodeOwner : AccountAddress)
+variable (symPerm : Bool)
 
 abbrev addEVM := @Operation.ADD .EVM
 
@@ -45,15 +48,31 @@ theorem EVM.step_add_to_step_add (gpos : 0 < gas) (symState : EVM.State):
       pc := symPc,
       gasAvailable := symGasAvailable,
       execLength := symExecLength,
-      executionEnv := {symState.executionEnv with code := symCode},
+      executionEnv := {symState.executionEnv with
+                  code := symCode,
+                  codeOwner := symCodeOwner,
+                  perm := symPerm},
+      accountMap := symAccounts
+      substate := {symState.substate with
+            accessedStorageKeys :=  symAccessedStorageKeys
+            refundBalance := symRefund
+           }
       returnData := symReturnData} =
   EvmYul.step_add
     {symState with
     stack := word₁ :: word₂ :: symStack
     gasAvailable := symGasAvailable - UInt256.ofNat gasCost
     pc := symPc,
-    executionEnv := {symState.executionEnv with code := symCode},
+    executionEnv := {symState.executionEnv with
+                  code := symCode,
+                  codeOwner := symCodeOwner,
+                  perm := symPerm},
+    accountMap := symAccounts
     returnData := symReturnData,
+    substate := {symState.substate with
+            accessedStorageKeys :=  symAccessedStorageKeys
+            refundBalance := symRefund
+           }
     execLength := symExecLength + 1} := by
       cases gas; contradiction
       simp [EVM.step_add, EVM.step]; rfl
@@ -65,14 +84,30 @@ theorem EVM.step_add_summary (gpos : 0 < gas) (symState : EVM.State):
       pc := symPc,
       gasAvailable := symGasAvailable,
       returnData := symReturnData,
-      executionEnv := {symState.executionEnv with code := symCode},
+      executionEnv := {symState.executionEnv with
+                    code := symCode,
+                    codeOwner := symCodeOwner,
+                    perm := symPerm},
+      accountMap := symAccounts
+      substate := {symState.substate with
+            accessedStorageKeys :=  symAccessedStorageKeys
+            refundBalance := symRefund
+           }
       execLength := symExecLength} =
     .ok {symState with
           stack := (word₁ + word₂) :: symStack,
           pc := UInt256.add symPc (.ofNat 1),
           gasAvailable := symGasAvailable - UInt256.ofNat gasCost,
           returnData := symReturnData,
-          executionEnv := {symState.executionEnv with code := symCode},
+          executionEnv := {symState.executionEnv with
+                        code := symCode,
+                        codeOwner := symCodeOwner,
+                        perm := symPerm},
+          accountMap := symAccounts
+          substate := {symState.substate with
+            accessedStorageKeys :=  symAccessedStorageKeys
+            refundBalance := symRefund
+           }
           execLength := symExecLength + 1} := by
   rw [EVM.step_add_to_step_add]; rfl; assumption
 
@@ -125,14 +160,30 @@ theorem X_add_summary (enoughGas : GasConstants.Gverylow < symGasAvailable.toNat
     pc := .ofNat 0,
     execLength := symExecLength,
     gasAvailable := symGasAvailable,
-    executionEnv := {symState.executionEnv with code := ⟨#[(0x1 : UInt8)]⟩}
+    executionEnv := {symState.executionEnv with
+                  code := ⟨#[(0x1 : UInt8)]⟩,
+                  codeOwner := symCodeOwner,
+                  perm := symPerm},
+    accountMap := symAccounts
+    substate := {symState.substate with
+            accessedStorageKeys :=  symAccessedStorageKeys
+            refundBalance := symRefund
+           }
     returnData := symReturnData} =
   Except.ok (.success {symState with
         stack := (word₁ + word₂) :: symStack,
         pc := .ofNat 1,
         gasAvailable := symGasAvailable - .ofNat GasConstants.Gverylow,
-        executionEnv := {symState.executionEnv with code := ⟨#[(0x1 : UInt8)]⟩},
+        executionEnv := {symState.executionEnv with
+                  code := ⟨#[(0x1 : UInt8)]⟩,
+                  codeOwner := symCodeOwner,
+                  perm := symPerm},
+        accountMap := symAccounts
         returnData := ByteArray.empty,
+        substate := {symState.substate with
+            accessedStorageKeys :=  symAccessedStorageKeys
+            refundBalance := symRefund
+           }
         execLength := symExecLength + 2} ByteArray.empty):= by
   cases g_case : symGasAvailable.toNat; rw [g_case] at enoughGas; contradiction
   case succ g_pos =>
@@ -146,7 +197,7 @@ theorem X_add_summary (enoughGas : GasConstants.Gverylow < symGasAvailable.toNat
   split; contradiction
   case h_2 evm _ stateOk =>
   have gPos : (0 < g_pos) := by aesop (add simp [GasConstants.Gverylow]) (add safe (by omega))
-  have step_rw := (EVM.step_add_summary word₁ word₂ g_pos GasConstants.Gverylow symStack (.ofNat 0) symGasAvailable symExecLength symReturnData ⟨#[(0x1 : UInt8)]⟩ gPos evm)
+  have step_rw := (EVM.step_add_summary word₁ word₂ g_pos GasConstants.Gverylow symStack (.ofNat 0) symGasAvailable symRefund symExecLength symReturnData ⟨#[(0x1 : UInt8)]⟩ symAccessedStorageKeys symAccounts symCodeOwner symPerm gPos evm)
   cases stateOk; rw [←EVM.step_add, step_rw]; simp [Except.instMonad, Except.bind]
   rw [X_bad_pc] <;> aesop (add simp [GasConstants.Gverylow]) (add safe (by omega))
 
