EvmEquivalence/Summaries/SstoreSummary.lean
@@ -1,0 +1,248 @@
+import EvmYul.EVM.Semantics
+import EvmYul.EVM.GasConstants
+--import EvmEquivalence.Summaries.StopSummary
+import EvmEquivalence.Interfaces.EvmYulInterface
+
+open EvmYul
+open EVM
+open EvmYul.State
+
+namespace SstoreSummary
+
+section
+
+variable (gas gasCost : ℕ)
+variable (symStack : Stack UInt256)
+variable (symPc symGasAvailable symRefund key value : UInt256)
+variable (symExecLength : ℕ)
+variable (symReturnData symCode : ByteArray)
+variable (symAccessedStorageKeys : Batteries.RBSet (AccountAddress × UInt256) Substate.storageKeysCmp)
+variable (symAccounts : AccountMap)
+variable (symCodeOwner : AccountAddress)
+variable (symPerm : Bool)
+
+@[simp]
+abbrev sstoreEVM := @Operation.SSTORE .EVM
+
+@[simp]
+abbrev sstore_instr : Option (Operation .EVM × Option (UInt256 × Nat)) :=
+  some ⟨sstoreEVM, none⟩
+
+@[simp]
+abbrev EVM.step_sstore : Transformer :=
+  EVM.step false gas gasCost sstore_instr
+
+@[simp]
+abbrev EvmYul.step_sstore : Transformer :=
+  EvmYul.step false sstoreEVM
+
+/--
+Theorem needed to bypass the `private` attribute of `EVM.dispatchBinaryStateOp`
+ -/
+theorem sstore_bypass_private (symState : EVM.State):
+  let ss := {symState with
+  stack := key :: value :: symStack,
+  pc := symPc
+  gasAvailable := symGasAvailable,
+  executionEnv := {symState.executionEnv with
+                  code := symCode,
+                  codeOwner := symCodeOwner
+                  perm := symPerm},
+  substate := {symState.substate with
+               accessedStorageKeys :=  symAccessedStorageKeys
+               refundBalance := symRefund}
+  returnData := symReturnData,
+  execLength := symExecLength,
+  accountMap := symAccounts}
+  EvmYul.step_sstore ss =
+  EVM.binaryStateOp false EvmYul.State.sstore ss := rfl
+
+@[simp]
+def accountMap_sstore (symState : EvmYul.State) (key value : UInt256) : AccountMap :=
+  let Iₐ := symState.executionEnv.codeOwner
+  let ownerAcc := (State.lookupAccount symState Iₐ)
+  match ownerAcc with
+  | none => symState.accountMap
+  | some ownerAcc =>
+    symState.accountMap.insert Iₐ (Account.updateStorage (ownerAcc) key value)
+
+@[simp]
+def accessedStorageKeys_sstore (symState : EvmYul.State) (key : UInt256) :=
+  let Iₐ := symState.executionEnv.codeOwner
+  let ownerAcc := (State.lookupAccount symState Iₐ)
+  match ownerAcc with
+  | none => symState.substate.accessedStorageKeys
+  | some _ => symState.substate.accessedStorageKeys.insert ⟨Iₐ, key⟩
+
+-- From EvmYul.StateOps.sstore
+@[local simp]
+def Aᵣ_sstore (symState: EvmYul.State) (key val : UInt256) : UInt256 :=
+    let Iₐ := symState.executionEnv.codeOwner
+  let { storage := σ_Iₐ, .. } := symState.accountMap.find! Iₐ
+  let { storage := σ₀_Iₐ, .. } := symState.σ₀.find! Iₐ
+  let v₀ := σ₀_Iₐ.findD key ⟨0⟩
+  let v := σ_Iₐ.findD key ⟨0⟩
+  let v' := val
+
+  let r_dirtyclear : ℤ :=
+    if v₀ ≠ .ofNat 0 && v = .ofNat 0 then - GasConstants.Rsclear else
+    if v₀ ≠ .ofNat 0 && v' = .ofNat 0 then GasConstants.Rsclear else
+    0
+
+  let r_dirtyreset : ℤ :=
+    if v₀ = v' && v₀ = .ofNat 0 then GasConstants.Gsset - GasConstants.Gwarmaccess else
+    if v₀ = v' && v₀ ≠ .ofNat 0 then GasConstants.Gsreset - GasConstants.Gwarmaccess else
+    0
+
+  let ΔAᵣ : ℤ :=
+    if v ≠ v' && v₀ = v && v' = .ofNat 0 then GasConstants.Rsclear else
+    if v ≠ v' && v₀ ≠ v then r_dirtyclear + r_dirtyreset else
+    0
+
+  let Iₐ := symState.executionEnv.codeOwner
+  let ownerAcc := (State.lookupAccount symState Iₐ)
+  match ownerAcc with
+  | none => symState.substate.refundBalance
+  | some _ =>
+    match ΔAᵣ with
+        | .ofNat n => symState.substate.refundBalance + .ofNat n
+        | .negSucc n => symState.substate.refundBalance - .ofNat n - ⟨1⟩
+
+theorem sstore_summary (symState : EvmYul.State) (key value : UInt256):
+  let ss := {symState with
+             executionEnv := {symState.executionEnv with
+                  code := symCode,
+                  codeOwner := symCodeOwner
+                  perm := symPerm},
+             substate := {symState.substate with
+                          accessedStorageKeys :=  symAccessedStorageKeys
+                          refundBalance := symRefund}
+             accountMap := symAccounts}
+  State.sstore ss key value =
+  {ss with
+    accountMap := accountMap_sstore ss key value,
+    substate.accessedStorageKeys := accessedStorageKeys_sstore ss key,
+    substate.refundBalance := Aᵣ_sstore ss key value} := by
+  cases cco: (symState.lookupAccount symState.executionEnv.codeOwner)
+  all_goals aesop (add simp [sstore, Aᵣ_sstore, Option.option, lookupAccount])
+
+theorem EvmYul.step_sstore_summary (symState : EVM.State):
+  let ss := {symState with
+    stack := key :: value :: symStack,
+    pc := symPc
+    gasAvailable := symGasAvailable,
+    executionEnv := {symState.executionEnv with
+                  code := symCode,
+                  codeOwner := symCodeOwner
+                  perm := symPerm},
+    substate := {symState.substate with
+                 accessedStorageKeys :=  symAccessedStorageKeys
+                 refundBalance := symRefund}
+    returnData := symReturnData,
+    execLength := symExecLength,
+    accountMap := symAccounts}
+  EvmYul.step_sstore ss =
+  .ok {ss with
+    stack := symStack,
+    pc := symPc + .ofNat 1
+    accountMap := accountMap_sstore ss.toState key value
+    substate.accessedStorageKeys := accessedStorageKeys_sstore ss.toState key
+    substate.refundBalance := Aᵣ_sstore ss.toState key value} := by
+  simp [sstore_bypass_private, binaryStateOp, Stack.pop2, Id.run, State.replaceStackAndIncrPC, State.incrPC]
+  aesop (add simp [sstore_summary])
+
+theorem EVM.step_sstore_summary (gas_pos : 0 < gas) (symState : EVM.State):
+  let ss := {symState with
+    stack := key :: value :: symStack,
+    pc := symPc
+    gasAvailable := symGasAvailable,
+    executionEnv := {symState.executionEnv with
+                  code := symCode,
+                  codeOwner := symCodeOwner
+                  perm := true},
+    substate := {symState.substate with
+                 accessedStorageKeys :=  symAccessedStorageKeys
+                 refundBalance := symRefund}
+    returnData := symReturnData,
+    execLength := symExecLength,
+    accountMap := symAccounts}
+  EVM.step_sstore gas gasCost ss =
+    .ok {ss with
+          stack := symStack,
+          pc := symPc + (.ofNat 1),
+          gasAvailable := symGasAvailable - UInt256.ofNat gasCost,
+          accountMap := accountMap_sstore ss.toState key value
+          substate := {ss.substate with
+            accessedStorageKeys := accessedStorageKeys_sstore ss.toState key
+            refundBalance := Aᵣ_sstore ss.toState key value
+           }
+          execLength := symExecLength + 1} := by
+  cases gas; contradiction
+  simp [step_sstore, EVM.step]
+  have srw := EvmYul.step_sstore_summary symStack symPc (symGasAvailable - UInt256.ofNat gasCost) symRefund key value (symExecLength + 1) symReturnData symCode
+  simp [EvmYul.step_sstore, Operation.SSTORE] at srw; aesop
+
+@[simp]
+theorem decode_singleton_sstore :
+  decode ⟨#[0x55]⟩ (.ofNat 0) = some ⟨sstoreEVM, none⟩ := rfl
+
+@[simp]
+theorem memoryExpansionCost_sstore (symState : EVM.State) :
+  memoryExpansionCost symState sstoreEVM = 0 := by
+  simp [memoryExpansionCost, memoryExpansionCost.μᵢ']
+
+/--
+TODO: Generalize to `C'`
+ -/
+theorem Csstore_pos (symState : EVM.State) : 99 < Csstore symState := by
+  aesop (add simp [Csstore, GasConstants.Gwarmaccess, GasConstants.Gsset, GasConstants.Gsreset])
+
+theorem X_sstore_summary (symState : EVM.State)
+                         (symStack_ok : symStack.length < 1024)
+                         (gasStippend : GasConstants.Gcallstipend < symGasAvailable.toNat):
+  let ss := {symState with
+    stack := key :: value :: symStack,
+    pc := .ofNat 0
+    gasAvailable := symGasAvailable,
+    executionEnv := {symState.executionEnv with
+                  code := ⟨#[(0x55 : UInt8)]⟩,
+                  codeOwner := symCodeOwner
+                  perm := true},
+    substate := {symState.substate with
+                 accessedStorageKeys :=  symAccessedStorageKeys
+                 refundBalance := symRefund}
+    returnData := symReturnData,
+    execLength := symExecLength,
+    accountMap := symAccounts}
+  Csstore ss < symGasAvailable.toNat →
+  X false symGasAvailable.toNat ss =
+  .ok (.success {ss with
+          stack := symStack,
+          pc := .ofNat 1,
+          gasAvailable := symGasAvailable - (.ofNat (Csstore ss)),
+          accountMap := accountMap_sstore ss.toState key value
+          substate := {ss.substate with
+            accessedStorageKeys := accessedStorageKeys_sstore ss.toState key
+            refundBalance := Aᵣ_sstore ss.toState key value
+           }
+          returnData := .empty,
+          execLength := symExecLength + 2} .empty) := by
+  intro ss enoughGas
+  have gavail_pos := Nat.lt_trans (Csstore_pos ss) enoughGas
+  cases g_case : symGasAvailable.toNat; rw [g_case] at gavail_pos; contradiction
+  case succ g_pos =>
+  simp [X, C', δ]
+  have lt_fls_rw {n m : ℕ} (_ : n < m) : (m < n) = False := by
+    simp; apply Nat.ge_of_not_lt; simp; omega
+  simp [ss, (lt_fls_rw enoughGas), α, (lt_fls_rw symStack_ok)]
+  have g_rw : (symGasAvailable.toNat ≤ GasConstants.Gcallstipend) = False := by aesop
+  simp [g_rw]; split; contradiction; next evm cost stateOk =>
+  have step_rw := (EVM.step_sstore_summary g_pos (Csstore evm) symStack (.ofNat 0)
+    symGasAvailable symRefund key value symExecLength symReturnData ⟨#[(0x55 : UInt8)]⟩
+    symAccessedStorageKeys symAccounts symCodeOwner (by omega) evm)
+  cases stateOk; simp at step_rw; rw [step_rw]; simp [Except.instMonad, Except.bind]
+  rw [X_bad_pc] <;> aesop (add safe (by omega))
+
+end
+
+end SstoreSummary
