EvmEquivalence/Equivalence/README.md
@@ -1,0 +1,91 @@
+# Opcode Equivalence
+
+This folder contains the equivalence proofs for opcode execution between the [`EvmYul`](https://github.com/nethermindEth/EVMYulLean/)
+and [`KEVM`](https://github.com/runtimeverification/evm-semantics) models.
+
+The proofs follow the following structure.
+
+## Proof sketch
+
+K rewrite rules are encoded as constructors of the inductive type `Rewrites` found in [Rewrite.lean](../KEVM2Lean/Rewrite.lean).
+That is, each constructor of `Rewrites` is a K rewrite rule. In particular, these K rewrite rules are generated from the [`KEVM` summaries](https://github.com/runtimeverification/evm-semantics/tree/master/kevm-pyk/src/kevm_pyk/kproj/evm-semantics/summaries).
+So the rewrite rules in `Rewrites` already encapsulate the computational content of executing an opcode in `KEVM`.
+
+Given this, let's understand the anatomy of a Lean-generated rewrite rule.
+
+### Anatomy of a rewrite rule
+
+Rewrite rules are comprised of
+- A left-hand side (lhs): `KEVM` state prior to the execution of an opcode. Also known as prestate.
+- A right-hand side (rhs): `KEVM` state derived from the execution of an opcode on the lhs. Also known as poststate.
+- All the variables involved in the definition of the lhs and rhs.
+- All the conditions that give meaning to the variables present in the lhs and rhs.
+
+Structurally we only need the first three items to make a rewrite rule type-check.
+The actual meaning of rewrite rules is encoded in all these conditions named `defn_Val*`.
+
+The structure of Lean-generated rewrite rules is as follows:
+```Lean
+inductive Rewrites : SortGeneratedTopCell → SortGeneratedTopCell → Prop where
+| NAME_OF_THE_RULE
+  {Var : CustomType} -- Variables are declared as implicit
+  ...                 -- A bunch more variables
+  (defn_Valn : f other_variables = some Valn) -- The meaning of the `_Valn` is explicitly given
+  ...                 -- A bunch more conditions
+  : Rewrites LHS RHS  -- Given all the conditions (`defn_Val*`) above, we can state LHS => RHS
+```
+
+Here `LHS` and `RHS` are representations of the `KEVM` pre and post states with the appropriate structure given by the `defn_Val*` conditions.
+
+### Proper definition of pre and post states
+
+The first step in all proofs is to have a precise definition of `LHS` and `RHS`.
+The naming convention is `opcode?HS` for each (e.g. `addLHS` for the prestate of the `ADD` opcode).
+
+Note that for these definitions we don't need any of the `defn_Val*` conditions yet, since we only care about the structural content of both states. That is, we don't need to know yet how the variables in these definitions relate to each other.
+
+#### Theorems-as-tests
+
+Once we have a definition of the `LHS` and `RHS` we want to test them and make sure they are the right ones.
+To this end, we can prove a theorem stating that, indeed, given all the `defn_Val*` preconditions, `Rewrites opcodeLHS opcodeRHS` holds.
+
+The general name for that theorem is `rw_opcodeLHS_opcodeRHS`.
+
+### Projecting `KEVM` states into `EvmYul`
+
+The next step is to reflect the resulting `EvmYul` state after transforming the `LHS` and `RHS` via the `stateMap` function.
+The `stateMap` function is defined in [`StateMap.lean`](../StateMap.lean).
+
+This reflection is done through the `opcode_prestate_equiv` and `opcode_poststate_equiv` theorems for the `opcodeLHS` and `opcodeRHS` respectively.
+These theorems are mostly structural, especially the `opcodeLHS`. However, the `opcode_poststate_equiv` is used to specify further what are the recorded effects of executing `opcode` in `KEVM`.
+
+To exemplify what this means, consider `add_poststate_equiv` in [`AddEquivalence.lean`](./AddEquivalence.lean).
+
+We have that the structural translation of the `PC_CELL` of `addRHS` into an `EvmYul` state is `pc := intMap _Val5`.
+That is, mapping the value of `_Val5` into a `UInt256`.
+However, as per `(defn_Val5 : «_+Int_» PC_CELL 1 = some _Val5)` and the definition of `«_+Int_»` found in [`FuncInterface.lean`](../Interfaces/FuncInterface.lean),
+we know that the value of `_Val5` is `PC_CELL + 1`.
+
+Hence, we will state `pc := intMap («_+Int'_» PC_CELL 1)` instead of `pc := intMap _Val5`. For more details on `«_+Int_»`, `«_+Int'_»` or more functions visit [`FuncInterface.lean`](../Interfaces/FuncInterface.lean).
+
+### Final proofs
+
+The `EvmYul` functions that reflect the semantics of executing an opcode are `EVM.step` and `X` found in [`EvmYul/EVM/Semantics.lean`](https://github.com/NethermindEth/EVMYulLean/blob/main/EvmYul/EVM/Semantics.lean).
+Since the full effects of opcode execution are separated between the two functions (for instance, `step` doesn't assign gas costs), we have one theorem for each function stating broadly the same.
+
+The statement is, for `f` being `EVM.step` or `EVM.X`:
+> Given the `KEVM` prestate `LHS`, `f (stateMap LHS) = stateMap RHS`
+That is, mapping the `KEVM` prestate to `EvmYul` and executing either `EVM.step` or `EVM.X` gives us the mapped `KEVM` poststate.
+
+A number of additional hypotheses from the `defn_Val*` is added to each theorem. Revisiting and sanity-checking these hypotheses is worthwhile.
+The vast majority of them stem from the fact that [`KEVM` summaries](https://github.com/runtimeverification/evm-semantics/tree/master/kevm-pyk/src/kevm_pyk/kproj/evm-semantics/summaries)
+assume that the `LHS` is a valid `KEVM` state. This means that conditions such as `PC_CELL < 2^256` are not enforced by the summaries and
+therefore need to be added as assumptions to obtain equivalence.
+
+These assumptions are present in the `KEVM` semantics, but they are enforced before triggering opcode execution.
+That is, the assumptions are not present in the rewrite rule of the opcodes, but in rewrite rules leading to opcode execution.
+
+### Future work
+
+Notably, these proofs are only in one direction. Namely, we show that if `KEVM` computes something, `EvmYul` agrees with a
+translation of that computation. It remains to prove the converse: that `KEVM` agrees with a translation of what `EvmYul` computes.
