EvmEquivalence/Interfaces/README.md
@@ -6,5 +6,33 @@ This folder contains interfaces to reason with the EvmYul and KEVM models.
 
 - [`EvmYulInterface`](./EvmYulInterface.lean): Interface for the EvmYul model
 - [`FuncInterface`](./FuncInterface.lean): Interface for dealing with generated KEVM functions
-- [`GasInterface`](./GasInterface.lean): Interface for the `«_<_>_SCHEDULE_Int_ScheduleConst_Schedule»` function
+- [`GasInterface`](./GasInterface.lean): Interface for the `«_<_>_SCHEDULE_Int_ScheduleConst_Schedule»` and `«_<<_>>_SCHEDULE_Bool_ScheduleFlag_Schedule»` functions
 - [`Tactics`](./Tactics.lean): Tactics to help with the [`GasInterface.lean`](./GasInterface.lean) proofs
+- [`Axioms`](./Axioms.lean): Axiomatization of the state mapping
+
+## Axiomatic mapping
+
+The file [`Axioms.lean`](./Axioms.lean) declares the exsistence of functions that convert `KEVM` maps into `EvmYul` ones.
+
+The reason for this axiomatization is twofold.
+
+1. Unimplemented maps in the K Lean 4 backend:
+   K maps are currently undefined in the Lean 4 generated code. We still have to come up with a suitable-enough implementation of K
+   maps that preserve the original semantics.
+
+   Note that this is tricky given that K maps have to be defined inside of a `mutual` inductive block, which limits the options
+   available to prevent crashing with Lean's positivity checker.
+   A clear disadvantage of this is that we cannot (apparently) use `FinMap` as our map implementation.
+2. Non reasoning-friendly maps in the `EvmYul` model:
+   Currently, the `EvmYul` model is more geared towards execution than reasoning.
+   This means that the map representation is not the most optimal for reasoning, and a more reasoning-friendly interface could be
+   provided in the future. This is an argument in favor of not commiting (yet) to a K map representation tailored to play well with
+   the current `EvmYul` maps, but this argument could change in the future.
+
+## Axioms as pre-theorems
+
+Given that we're axiomatizing part of the state translation, properties on the axiomatic parts need to be provided.
+How the axiomatic parts of the state mapping are _needed_ to behave is laid out in the `Axioms` namespace at the end of the [`StateMap.lean`](../StateMap.lean) file.
+
+These axioms establish the correspondence between the mapped data and the functions in the `EvmYul` map implementation.
+Once we have a clear implementation of K maps in Lean, all these axioms should become theorems.
