README.md
@@ -18,10 +18,10 @@ To this end, the K framework allows for the generation of Lean 4 code representi
 Under [EvmEquivalence](./EvmEquivalence) we have the following structure:
 * [KEVM2Lean](./EvmEquivalence/KEVM2Lean): K-generated Lean 4 code with modifications
 * [Interfaces](./EvmEquivalence/Interfaces): Proving interfaces to interact with the K-generated Lean 4 code
+* [Summaries](./EvmEquivalence/Summaries): Summaries of relevant functions from the `EvmYul` model
+* [Equivalence](./EvmEquivalence/Equivalence): Proof of equivalence between the models in a per-opcode basis
 * [Utils](./EvmEquivalence/Utils): Useful results for the proving
-* [Summaries.lean](./EvmEquivalence/Summaries.lean): Summaries of relevant functions from the `EvmYul` model
 * [StateMap.lean](./EvmEquivalence/StateMap.lean): Function mapping `KEVM` states to `EvmYul` states
-* [AddEquivalence.lean](./EvmEquivalence/AddEquivalence.lean): Proof of equivalence between the models for the `ADD` opcode
 
 ## Lean 4 Code Generation
 
